

IT5005 Artificial Intelligence

Matrix Calculus

Sirigina Rajendra Prasad

Matrix Calculus (Denominator Layout)

$$\bullet \text{ Let } \mathbf{y} = \begin{bmatrix} y_1 \\ y_2 \\ \vdots \\ y_r \end{bmatrix}_{r \times 1} \quad \mathbf{x} = \begin{bmatrix} x_1 \\ x_2 \\ \vdots \\ x_n \end{bmatrix}_{n \times 1} \quad \mathbf{X} = \begin{bmatrix} x_{11} & \cdots & x_{1n} \\ \vdots & \ddots & \vdots \\ x_{m1} & \cdots & x_{mn} \end{bmatrix}_{m \times n}$$

$$\frac{\partial \mathbf{y}}{\partial \mathbf{x}} = \begin{bmatrix} \frac{\partial y}{\partial x_1} \\ \vdots \\ \frac{\partial y}{\partial x_n} \end{bmatrix}_{n \times 1} \qquad \frac{\partial \mathbf{y}}{\partial \mathbf{X}} = \begin{bmatrix} \frac{\partial y}{\partial x_{11}} & \cdots & \frac{\partial y}{\partial x_{1n}} \\ \vdots & \ddots & \vdots \\ \frac{\partial y}{\partial x_{m1}} & \cdots & \frac{\partial y}{\partial x_{mn}} \end{bmatrix}_{m \times n}$$

$$\frac{\partial \mathbf{y}}{\partial \mathbf{x}} = \begin{bmatrix} \frac{\partial y_1}{\partial x_1} & \cdots & \frac{\partial y_r}{\partial x_1} \\ \vdots & \ddots & \vdots \\ \frac{\partial y_1}{\partial x_n} & \cdots & \frac{\partial y_r}{\partial x_n} \end{bmatrix}_{n \times r} \qquad \frac{\partial \mathbf{y}}{\partial \mathbf{X}} = \begin{bmatrix} \frac{\partial y_1}{\partial x_{11}} & \cdots & \frac{\partial y_1}{\partial x_{1n}} \\ \vdots & \ddots & \vdots \\ \frac{\partial y_1}{\partial x_{m1}} & \cdots & \frac{\partial y_1}{\partial x_{mn}} \end{bmatrix} \cdot \begin{bmatrix} \frac{\partial y_r}{\partial x_{11}} & \cdots & \frac{\partial y_r}{\partial x_{1n}} \\ \vdots & \ddots & \vdots \\ \frac{\partial y_r}{\partial x_{m1}} & \cdots & \frac{\partial y_r}{\partial x_{mn}} \end{bmatrix}_{m \times n \times r}$$

Matrix Calculus (Denominator Layout)

- Vector-by-Vector Identities:

Condition	Expression	Numerator layout, i.e. by \mathbf{y} and \mathbf{x}^T	Denominator layout, i.e. by \mathbf{y}^T and \mathbf{x}
\mathbf{a} is not a function of \mathbf{x}	$\frac{\partial \mathbf{a}}{\partial \mathbf{x}} =$	$\mathbf{0}$	
	$\frac{\partial \mathbf{x}}{\partial \mathbf{x}} =$	\mathbf{I}	
\mathbf{A} is not a function of \mathbf{x}	$\frac{\partial \mathbf{A} \mathbf{x}}{\partial \mathbf{x}} =$	\mathbf{A}	\mathbf{A}^T
\mathbf{A} is not a function of \mathbf{x}	$\frac{\partial \mathbf{x}^T \mathbf{A}}{\partial \mathbf{x}} =$	\mathbf{A}^T	\mathbf{A}
a is not a function of \mathbf{x} , $\mathbf{u} = \mathbf{u}(\mathbf{x})$	$\frac{\partial a \mathbf{u}}{\partial \mathbf{x}} =$	$a \frac{\partial \mathbf{u}}{\partial \mathbf{x}}$	
$v = v(\mathbf{x})$, \mathbf{a} is not a function of \mathbf{x}	$\frac{\partial v \mathbf{a}}{\partial \mathbf{x}} =$	$\mathbf{a} \frac{\partial v}{\partial \mathbf{x}}$	$\frac{\partial v}{\partial \mathbf{x}} \mathbf{a}^T$
$v = v(\mathbf{x})$, $\mathbf{u} = \mathbf{u}(\mathbf{x})$	$\frac{\partial v \mathbf{u}}{\partial \mathbf{x}} =$	$v \frac{\partial \mathbf{u}}{\partial \mathbf{x}} + \mathbf{u} \frac{\partial v}{\partial \mathbf{x}}$	$v \frac{\partial \mathbf{u}}{\partial \mathbf{x}} + \frac{\partial v}{\partial \mathbf{x}} \mathbf{u}^T$
\mathbf{A} is not a function of \mathbf{x} , $\mathbf{u} = \mathbf{u}(\mathbf{x})$	$\frac{\partial \mathbf{A} \mathbf{u}}{\partial \mathbf{x}} =$	$\mathbf{A} \frac{\partial \mathbf{u}}{\partial \mathbf{x}}$	$\frac{\partial \mathbf{u}}{\partial \mathbf{x}} \mathbf{A}^T$
$\mathbf{u} = \mathbf{u}(\mathbf{x})$, $\mathbf{v} = \mathbf{v}(\mathbf{x})$	$\frac{\partial (\mathbf{u} + \mathbf{v})}{\partial \mathbf{x}} =$	$\frac{\partial \mathbf{u}}{\partial \mathbf{x}} + \frac{\partial \mathbf{v}}{\partial \mathbf{x}}$	
$\mathbf{u} = \mathbf{u}(\mathbf{x})$	$\frac{\partial \mathbf{g}(\mathbf{u})}{\partial \mathbf{x}} =$	$\frac{\partial \mathbf{g}(\mathbf{u})}{\partial \mathbf{u}} \frac{\partial \mathbf{u}}{\partial \mathbf{x}}$	$\frac{\partial \mathbf{u}}{\partial \mathbf{x}} \frac{\partial \mathbf{g}(\mathbf{u})}{\partial \mathbf{u}}$
$\mathbf{u} = \mathbf{u}(\mathbf{x})$	$\frac{\partial \mathbf{f}(\mathbf{g}(\mathbf{u}))}{\partial \mathbf{x}} =$	$\frac{\partial \mathbf{f}(\mathbf{g})}{\partial \mathbf{g}} \frac{\partial \mathbf{g}(\mathbf{u})}{\partial \mathbf{u}} \frac{\partial \mathbf{u}}{\partial \mathbf{x}}$	$\frac{\partial \mathbf{u}}{\partial \mathbf{x}} \frac{\partial \mathbf{g}(\mathbf{u})}{\partial \mathbf{u}} \frac{\partial \mathbf{f}(\mathbf{g})}{\partial \mathbf{g}}$

Chain Rule (Denominator Layout)

- \mathbf{g} is a vector-valued function with output vector of shape $m \times 1$
- \mathbf{f} is a column vector of shape $d \times 1$
- \mathbf{x} is a column vector of shape $n \times 1$

$$\underbrace{\frac{\partial \mathbf{g}(\mathbf{f})}{\partial \mathbf{x}}}_{n \times m} = \underbrace{\frac{\partial \mathbf{f}}{\partial \mathbf{x}}}_{n \times d} \underbrace{\frac{\partial \mathbf{g}(\mathbf{f})}{\partial \mathbf{f}}}_{d \times m}$$

Matrix Calculus: Matrix Identities

- Let $\mathbf{z} = W\mathbf{x}$, where $\mathbf{x} \in \mathbb{R}^{m \times 1}$, $W \in \mathbb{R}^{n \times m}$. Find $\frac{\partial \mathbf{z}}{\partial \mathbf{x}}$?

$$\frac{\partial \mathbf{z}}{\partial \mathbf{x}} = \begin{bmatrix} \frac{\partial z_1}{\partial x_1} & \cdots & \frac{\partial z_n}{\partial x_1} \\ \vdots & \ddots & \vdots \\ \frac{\partial z_1}{\partial x_m} & \cdots & \frac{\partial z_n}{\partial x_m} \end{bmatrix}$$

$$z_i = \sum_{k=1}^m W_{ik} x_k \Rightarrow \frac{\partial z_i}{\partial x_k} = W_{ik}$$

$$\Rightarrow \frac{\partial \mathbf{z}}{\partial \mathbf{x}} = \begin{bmatrix} W_{11} & \cdots & W_{n1} \\ \vdots & \ddots & \vdots \\ W_{1m} & \cdots & W_{nm} \end{bmatrix} = W^T$$

Matrix Calculus: Matrix Identities

- Let $\mathbf{z} = \mathbf{x}^T W$, where $\mathbf{x} \in \mathbb{R}^{m \times 1}$, $W \in \mathbb{R}^{m \times n}$. Find $\frac{\partial \mathbf{z}}{\partial \mathbf{x}}$?

$$\frac{\partial \mathbf{z}}{\partial \mathbf{x}} = \begin{bmatrix} \frac{\partial z_1}{\partial x_1} & \cdots & \frac{\partial z_n}{\partial x_1} \\ \vdots & \ddots & \vdots \\ \frac{\partial z_1}{\partial x_m} & \cdots & \frac{\partial z_n}{\partial x_m} \end{bmatrix}$$

$$z_i = \sum_{k=1}^m x_k W_{ki} \Rightarrow \frac{\partial z_i}{\partial x_j} = W_{ji}$$

$$\Rightarrow \frac{\partial \mathbf{z}}{\partial \mathbf{x}} = \begin{bmatrix} W_{11} & \cdots & W_{1n} \\ \vdots & \ddots & \vdots \\ W_{m1} & \cdots & W_{mn} \end{bmatrix} = W$$

Matrix Calculus: Matrix Identities

- Let $\mathbf{x} \in \mathbb{R}^{m \times 1}$ and $\mathbf{z} = g(\mathbf{x}) = \begin{bmatrix} g(x_1) \\ \vdots \\ g(x_m) \end{bmatrix}$, i.e., function g performs element-wise application for the vector \mathbf{x} . Find $\frac{\partial \mathbf{z}}{\partial \mathbf{x}}$?

$$\frac{\partial \mathbf{z}}{\partial \mathbf{x}} = \begin{bmatrix} \frac{\partial z_1}{\partial x_1} & \cdots & \frac{\partial z_m}{\partial x_1} \\ \vdots & \ddots & \vdots \\ \frac{\partial z_1}{\partial x_m} & \cdots & \frac{\partial z_m}{\partial x_m} \end{bmatrix} = \begin{bmatrix} \frac{\partial g(x_1)}{\partial x_1} & \cdots & \frac{\partial g(x_m)}{\partial x_1} \\ \vdots & \ddots & \vdots \\ \frac{\partial g(x_1)}{\partial x_m} & \cdots & \frac{\partial g(x_1)}{\partial x_m} \end{bmatrix}$$

$$= \begin{bmatrix} \frac{\partial g(x_1)}{\partial x_1} & \cdots & 0 \\ \vdots & \ddots & \vdots \\ 0 & \cdots & \frac{\partial g(x_1)}{\partial x_m} \end{bmatrix} = \mathbf{diag}[\mathbf{z}'] \quad \mathbf{z}' = g'(\mathbf{x}) = \begin{bmatrix} g'(x_1) \\ \vdots \\ g'(x_m) \end{bmatrix}$$

Matrix Calculus: Matrix Identities

- Let $\mathbf{f} = \mathbf{W}^T \mathbf{a}$, where $\mathbf{W} \in \mathbb{R}^{m \times n}$ and $\mathbf{a} \in \mathbb{R}^{m \times 1}$. Let $g(\mathbf{f}(\mathbf{W}))$ be a scalar function. Assuming denominator layout show that

$$\frac{\partial g(\mathbf{f}(\mathbf{W}))}{\partial \mathbf{W}} = \frac{\partial \mathbf{f}(\mathbf{W})}{\partial \mathbf{W}} \frac{\partial g(\mathbf{f})}{\partial \mathbf{f}} = \mathbf{a} \left(\frac{\partial g(\mathbf{f})}{\partial \mathbf{f}} \right)^T$$

Chain Rule in Denominator Layout:

$$\underbrace{\frac{\partial g(\mathbf{f}(\mathbf{W}))}{\partial \mathbf{W}}}_{m \times n} = \underbrace{\frac{\partial \mathbf{f}(\mathbf{W})}{\partial \mathbf{W}}}_{m \times n \times n} \underbrace{\frac{\partial g(\mathbf{f})}{\partial \mathbf{f}}}_{n \times 1}$$

$$\begin{aligned} \mathbf{a} &\in \mathbb{R}^{m \times 1} \\ \mathbf{W} &\in \mathbb{R}^{m \times n} \\ \mathbf{f} &\in \mathbb{R}^{n \times 1} \\ g(\mathbf{f}) &: \mathbb{R}^{n \times 1} \rightarrow \mathbb{R} \end{aligned}$$

- Proof:

➤ Let's start with $\frac{\partial g(\mathbf{f}(W))}{\partial W_{ij}}$, where W_{ij} is a scalar from i -th row and j -th column of matrix W

$$\underbrace{\frac{\partial g(\mathbf{f})}{\partial W_{ij}}}_{1 \times 1} = \underbrace{\frac{\partial \mathbf{f}(W)}{\partial W_{ij}}}_{1 \times n} \underbrace{\frac{\partial g(\mathbf{f})}{\partial \mathbf{f}}}_{n \times 1}$$

$$\begin{aligned} \mathbf{a} &\in \mathbb{R}^{m \times 1} \\ W &\in \mathbb{R}^{m \times n} \\ \mathbf{f} &\in \mathbb{R}^{n \times 1} \\ g(\mathbf{f}) &: \mathbb{R}^{n \times 1} \rightarrow \mathbb{R} \end{aligned}$$

- Proof (contd):

$$\frac{\partial g(\mathbf{f}(W))}{\partial W_{ij}} = \frac{\partial \mathbf{f}}{\partial W_{ij}} \frac{\partial g(\mathbf{f}(W))}{\partial \mathbf{f}}$$

$$\frac{\partial \mathbf{f}(W)}{\partial W_{ij}} = \left[\frac{\partial f_1(W)}{\partial W_{ij}} \quad \dots \quad \frac{\partial f_k(W)}{\partial W_{ij}} \quad \dots \quad \frac{\partial f_n(W)}{\partial W_{ij}} \right] \in \mathbb{R}^{1 \times n}$$

$$\mathbf{f} = W^T \mathbf{a}$$

$$\Rightarrow f_k = \sum_{l=1}^m W_{lk} a_l$$

k-th column of matrix W

$$\frac{\partial f_k(W)}{\partial W_{ij}} = \frac{\partial}{\partial W_{ij}} \left(\sum_{l=1}^m W_{lk} a_l \right)$$

$$= \begin{cases} a_i & \text{if } l = i \text{ and } k = j \\ 0 & \text{otherwise} \end{cases}$$

$$\Rightarrow \frac{\partial \mathbf{f}(W)}{\partial W_{ij}} = [0 \quad \dots \quad 0 \quad a_i \quad 0 \quad \dots \quad 0]$$



j - th element of the vector $\frac{\partial \mathbf{f}(W)}{\partial W_{ij}}$

$$\mathbf{a} \in \mathbb{R}^{m \times 1}$$

$$W \in \mathbb{R}^{m \times n}$$

$$\mathbf{f} \in \mathbb{R}^{n \times 1}$$

$$g(\mathbf{f}): \mathbb{R}^{n \times 1} \rightarrow \mathbb{R}$$

f_k : k -th element of vector \mathbf{f}

- Proof (contd):

$$\frac{\partial g(\mathbf{f}(W))}{\partial W_{ij}} = \frac{\partial \mathbf{f}(W)}{\partial W_{ij}} \frac{\partial g(\mathbf{f})}{\partial \mathbf{f}}$$

Let $\boldsymbol{\delta} = \frac{\partial g(\mathbf{f})}{\partial \mathbf{f}}$

δ_j : j -th element of the vector $\boldsymbol{\delta}$

$$\mathbf{a} \in \mathbb{R}^{m \times 1}$$

$$W \in \mathbb{R}^{m \times n}$$

$$\mathbf{f} \in \mathbb{R}^{n \times 1}$$

$$g(\mathbf{f}): \mathbb{R}^{n \times 1} \rightarrow \mathbb{R}$$

$$\frac{\partial g(\mathbf{f})}{\partial W_{ij}} = \frac{\partial \mathbf{f}(W)}{\partial W_{ij}} \frac{\partial g(\mathbf{f})}{\partial \mathbf{f}}$$

f_k : k -th element of vector \mathbf{f}

$$= [0 \quad \dots \quad 0 \quad a_i \quad 0 \quad \dots \quad 0] \boldsymbol{\delta}$$

$$= a_i \delta_j$$

- Proof (contd):

$$\frac{\partial g(\mathbf{f})}{\partial W_{ij}} = a_i \delta_j$$

$$\Rightarrow \frac{\partial g(\mathbf{f})}{\partial \mathbf{W}} = \begin{bmatrix} a_1 \delta_1 & \cdots & a_1 \delta_n \\ \vdots & \ddots & \vdots \\ a_m \delta_1 & \cdots & a_m \delta_n \end{bmatrix}$$

$$= \begin{bmatrix} a_1 \\ \vdots \\ a_m \end{bmatrix} [\delta_1 \quad \cdots \quad \delta_n]$$

$$= \mathbf{a} \boldsymbol{\delta}^T$$

$$\Rightarrow \frac{\partial g(\mathbf{f})}{\partial \mathbf{W}} = \mathbf{a} \left(\frac{\partial g(\mathbf{f})}{\partial \mathbf{f}} \right)^T$$

$$\mathbf{W} \in \mathbb{R}^{m \times n}$$

$$\mathbf{f} = \mathbf{W}^T \mathbf{a}$$